working on GeneralRec.v

src/GeneralRec.v
@@ -18,3 +18,81 @@ Set Implicit Arguments.
 Set Asymmetric Patterns.
 (* end hide *)
 
+Section mergeSort.
+  Variable A : Type.
+  Variable le : A -> A -> bool.
+
+  Fixpoint insert (x : A) (ls : list A) :=
+    match ls with
+    | nil => x :: nil
+    | y :: ls' => if le x y then x :: ls else y :: (insert x ls')
+    end.
+
+  Fixpoint merge (ls1 ls2 : list A) :=
+    match ls1 with
+    | nil => ls2
+    | h :: ls1' => insert h (merge ls1' ls2)
+    end.
+
+  Fixpoint split (ls : list A) : list A * list A :=
+    match ls with
+    | nil => (nil, nil)
+    | x :: nil => (ls, nil)
+    | x :: y :: ls' =>
+      let (ls1', ls2') := split ls' in
+      (x :: ls1', y :: ls2')
+    end.
+
+  (* Fixpoint mergeSort (ls : list A) := *)
+  (*   if (leb (length ls) 1) *)
+  (*   then ls *)
+  (*   else *)
+  (*     let (ls1, ls2) := split ls in *)
+  (*     merge (mergeSort ls1) (mergeSort ls2). *)
+  
+  
+  Inductive Acc' (A : Type) (R : A -> A -> Prop): A -> Prop :=
+  | Acc_intro' : forall x : A, (forall y : A, R y x -> Acc' R y) -> Acc' R x.
+  
+  CoInductive infiniteDecreasingChain A (R : A -> A -> Prop) : stream A -> Prop :=
+  | ChainCons : forall x y s, infiniteDecreasingChain R (Cons y s) -> R y x -> infiniteDecreasingChain R (Cons x (Cons y s)).
+
+  Lemma noBadChains' : forall A (R : A -> A -> Prop) x, Acc R x -> forall s, ~ infiniteDecreasingChain R (Cons x s).
+    intros. generalize dependent s. induction H.
+    intro s. intro Contra.
+    inversion Contra.
+    apply (H0 y H4 s0 H3).
+  Qed.
+  
+  
+  Theorem noBadChains : forall A (R : A -> A -> Prop), (forall a : A, Acc R a) -> forall s, ~ infiniteDecreasingChain R s.
+    destruct s. apply noBadChains'. eauto.
+  Qed.
+  
+  Check Fix.
+  
+  Definition lengthOrder (ls1 ls2 : list A) :=
+    length ls1 < length ls2.
+
+  Hint Constructors Acc.
+
+  Lemma lengthOrder_wf' : forall len ls, length ls <= len -> Acc lengthOrder ls.
+    unfold lengthOrder; induction len; crush.
+  Defined.
+
+  Theorem lengthOrder_wf : well_founded lengthOrder.
+    red; intro; eapply lengthOrder_wf'; eauto.
+  Defined.
+
+  Lemma split_wf : forall len ls, 2 <= length ls <= len
+                              -> let (ls1, ls2) := split ls in
+                                 lengthOrder ls1 ls /\ lengthOrder ls2 ls.
+  unfold lengthOrder; induction len; crush; do 2 (destruct ls; crush);
+                                                 destruct (le_lt_dec 2 (length ls));
+                                                 repeat (match goal with
+                                                         | [ _ : length ?E <2 |- _ ] => destruct E
+                                                         | [ _ : S (length ?E) < 2 |- _ ] => destruct E
+                                                         | [IH : _ |- context [split ?l] ] => specialize (IH L); destruct (split L); destruct IH
+                                                         end; crush).
+  
+  
